src/lean4/human_eval/problem_110.lean
@@ -32,6 +32,8 @@ let spec (result : String) :=
   let bool_result := ∃ exchange: List (Nat × Nat),
     let lst1_idxs := exchange.map (fun (a, b) => a)
     let lst2_idxs := exchange.map (fun (a, b) => b)
+    lst1_idxs.all (fun i => i < lst1.length) ∧
+    lst2_idxs.all (fun i => i < lst2.length) ∧
     lst1_idxs.Nodup ∧
     lst2_idxs.Nodup ∧
     ∀ i, i < lst1.length →
@@ -39,7 +41,7 @@ let spec (result : String) :=
       (i ∈ lst1_idxs →
         -- find the (a, b) in exchange where a = i
         let i_idx := (lst1_idxs.indexesOf i).head!
-        Even (lst2.get! i_idx))
+        Even (lst2.get! (lst2_idxs.get! i_idx)))
   (bool_result → result = "YES") ∧
   (result = "NO" → ¬ bool_result) ∧
   (result ≠ "YES" ∧ result ≠ "NO" → False)
