src/lean4/human_eval/problem_117.lean
@@ -37,11 +37,12 @@ let spec (result : List String) :=
     c ∉ ['A', 'E', 'I', 'O', 'U'] ∧
     c.isAlpha
   s.all (fun c => c = ' ' ∨ c.isAlpha) →
-  (s.length = 0 → result = []) ∧
   let words := s.splitOn " "
+  (result = [] ↔ (s.length = 0 ∨ words.all (fun word => (word.data.filter (fun c => is_consonant c)).length ≠ n))) ∧
   (result.length > 0 →
     let first_word := result[0]!
     first_word ∈ words ∧
+    (first_word.data.filter (fun c => is_consonant c)).length = n ∧
     let first_word_idx := words.indexOf first_word
     (∀ i, i < first_word_idx →
       (words[i]!.data.filter (fun c => is_consonant c)).length ≠ n) ∧
